WIP, proving intro-ghost, found valid ptr issue

coq/proof/SoundInfruleIntroGhost.v
@@ -36,12 +36,26 @@ Set Implicit Arguments.
 
 
 
-Lemma list_inb_false_app
+Lemma list_inb_false_app_inv
       X (xs0 xs1: list X) X_dec x
       (INB: list_inb X_dec (xs0 ++ xs1) x = false)
   :
     <<INB0: list_inb X_dec xs0 x = false>> /\
             <<INB1: list_inb X_dec xs1 x = false>>
+.
+Proof.
+  unfold NW.
+  unfold list_inb, is_some in *.
+  des_ifs_safe.
+  rewrite find_app in Heq. des_ifs.
+Qed.
+
+Lemma list_inb_false_app
+      X (xs0 xs1: list X) X_dec x
+      (INB0: list_inb X_dec xs0 x = false)
+      (INB1: list_inb X_dec xs1 x = false)
+  :
+    <<INB: list_inb X_dec (xs0 ++ xs1) x = false>>
 .
 Proof.
   unfold NW.
@@ -82,23 +96,45 @@ Proof.
   des_ifs.
 Qed.
 
-Definition cons_ghost (i0: id) (gv_src gv_tgt: GenericValue)
-           (inv0: InvState.Rel.t): InvState.Rel.t :=
-  InvState.Rel.mk (InvState.Unary.update_ghost
-                     (fun idgs => (i0, gv_src) :: idgs) inv0.(InvState.Rel.src))
-                  (InvState.Unary.update_ghost
-                     (fun idgs => (i0, gv_tgt) :: idgs) inv0.(InvState.Rel.tgt))
+Lemma list_inb_filter_map_cons
+      X (v: X) (vs: list X) (f: X -> option IdT.t)
+      idt0
+      (INB0: list_inb IdTSetFacts.eq_dec (f v) idt0 = false)
+      (INB1: list_inb IdTSetFacts.eq_dec
+                      (filter_map f vs) idt0 = false)
+  :
+    <<INB: list_inb IdTSetFacts.eq_dec
+                    (filter_map f (v :: vs)) idt0 = false>>
 .
+Proof.
+  ss.
+  compute in INB0.
+  compute in INB1.
+  compute.
+  des_ifs.
+Qed.
+
+Corollary list_inb_filter_map_cons_one
+      X (v w: X) (f: X -> option IdT.t) idt0
+      (INB0: list_inb IdTSetFacts.eq_dec (f v) idt0 = false)
+      (INB1: list_inb IdTSetFacts.eq_dec (f w) idt0 = false)
+  :
+    <<INB: list_inb IdTSetFacts.eq_dec (filter_map f [v; w]) idt0 = false>>
+.
+Proof.
+  eapply list_inb_filter_map_cons; eauto.
+Qed.
+
 
 Section CLEAR_IDTS.
 
   Lemma clear_idt_spec_id
         i0 idt0
         (CLEAR: proj_sumbool (IdTSetFacts.eq_dec i0 idt0) = false)
-        st_src invst0
+        st invst0
   :
-    <<EQ: InvState.Unary.sem_idT st_src invst0 i0 =
-          InvState.Unary.sem_idT st_src (InvState.Unary.clear_idt idt0 invst0) i0>>
+    <<EQ: InvState.Unary.sem_idT st invst0 i0 =
+          InvState.Unary.sem_idT st (InvState.Unary.clear_idt idt0 invst0) i0>>
   .
   Proof.
     red.
@@ -118,34 +154,13 @@ Section CLEAR_IDTS.
       des_bool. des_sumbool. clarify.
   Qed.
 
-  Lemma clear_idt_spec_inv_id
-        i0 idt0 st_src invst0
-        gv
-        (SOME: InvState.Unary.sem_idT st_src (InvState.Unary.clear_idt idt0 invst0) i0
-               = Some gv)
-        (NOTPHYSICAL: idt0.(fst) <> Tag.physical)
-    :
-      (* <<NOTIN: idt0 <> i0>> *)
-      <<CLEAR: proj_sumbool (IdTSetFacts.eq_dec i0 idt0) = false>>
-  .
-  Proof.
-    red.
-    unfold InvState.Unary.clear_idt in *. des_ifs_safe. ss.
-    unfold proj_sumbool. des_ifs_safe.
-    destruct t; ss.
-    - unfold InvState.Unary.sem_idT, InvState.Unary.sem_tag in *. ss.
-      rewrite lookup_AL_filter_spec in SOME. unfold negb, proj_sumbool in *. des_ifs.
-    - unfold InvState.Unary.sem_idT, InvState.Unary.sem_tag in *. ss.
-      rewrite lookup_AL_filter_spec in SOME. unfold negb, proj_sumbool in *. des_ifs.
-  Qed.
-
   Lemma clear_idt_spec_value
         v0 idt0
         (CLEAR: list_inb IdTSetFacts.eq_dec (ValueT.get_idTs v0) idt0 = false)
-        conf_src st_src invst0
+        conf st invst0
     :
-      <<EQ: InvState.Unary.sem_valueT conf_src st_src invst0 v0 =
-            InvState.Unary.sem_valueT conf_src st_src (InvState.Unary.clear_idt idt0 invst0) v0>>
+      <<EQ: InvState.Unary.sem_valueT conf st invst0 v0 =
+            InvState.Unary.sem_valueT conf st (InvState.Unary.clear_idt idt0 invst0) v0>>
   .
   Proof.
     red. unfold InvState.Unary.sem_valueT. des_ifs.
@@ -157,10 +172,10 @@ Section CLEAR_IDTS.
   Lemma clear_idt_spec_list_value
         vs0 idt0
         (CLEAR: list_inb IdTSetFacts.eq_dec (filter_map ValueT.get_idTs (List.map snd vs0)) idt0 = false)
-        conf_src st_src invst0
+        conf st invst0
     :
-      <<EQ: InvState.Unary.sem_list_valueT conf_src st_src invst0 vs0 =
-            InvState.Unary.sem_list_valueT conf_src st_src (InvState.Unary.clear_idt idt0 invst0) vs0>>
+      <<EQ: InvState.Unary.sem_list_valueT conf st invst0 vs0 =
+            InvState.Unary.sem_list_valueT conf st (InvState.Unary.clear_idt idt0 invst0) vs0>>
   .
   Proof.
     red. (* unfold InvState.Unary.sem_valueT. des_ifs. *)
@@ -185,10 +200,10 @@ Section CLEAR_IDTS.
   Lemma clear_idt_spec_expr
         x idt0
         (CLEAR: list_inb IdTSetFacts.eq_dec (Expr.get_idTs x) idt0 = false)
-        conf_src st_src invst0
+        conf st invst0
     :
-      <<EQ: InvState.Unary.sem_expr conf_src st_src invst0 x =
-            InvState.Unary.sem_expr conf_src st_src (InvState.Unary.clear_idt idt0 invst0) x>>
+      <<EQ: InvState.Unary.sem_expr conf st invst0 x =
+            InvState.Unary.sem_expr conf st (InvState.Unary.clear_idt idt0 invst0) x>>
   .
   Proof.
     red.
@@ -229,19 +244,19 @@ Section CLEAR_IDTS.
   Lemma clear_idt_spec_expr_set
         ep eps idt0
         (CLEAR: ExprPairSet.In ep (ExprPairSet.clear_idt idt0 eps))
-        conf_src st_src invst0
+        conf st invst0
     :
-      <<EQ: InvState.Unary.sem_expr conf_src st_src invst0 ep.(fst) =
-            InvState.Unary.sem_expr conf_src st_src (InvState.Unary.clear_idt idt0 invst0) ep.(fst)>> /\
-            <<EQ: InvState.Unary.sem_expr conf_src st_src invst0 ep.(snd) =
-                  InvState.Unary.sem_expr conf_src st_src (InvState.Unary.clear_idt idt0 invst0) ep.(snd)>>
+      <<EQ: InvState.Unary.sem_expr conf st invst0 ep.(fst) =
+            InvState.Unary.sem_expr conf st (InvState.Unary.clear_idt idt0 invst0) ep.(fst)>> /\
+            <<EQ: InvState.Unary.sem_expr conf st invst0 ep.(snd) =
+                  InvState.Unary.sem_expr conf st (InvState.Unary.clear_idt idt0 invst0) ep.(snd)>>
   .
   Proof.
     unfold NW. destruct ep; ss.
     unfold ExprPairSet.clear_idt in *.
     apply ExprPairSetFacts.filter_iff in CLEAR; [| solve_compat_bool ].
     repeat (des; des_bool).
-    apply list_inb_false_app in CLEAR0. des. ss.
+    apply list_inb_false_app_inv in CLEAR0. des. ss.
     erewrite <- clear_idt_spec_expr; eauto.
     erewrite <- clear_idt_spec_expr; eauto.
   Qed.
@@ -285,7 +300,7 @@ Section CLEAR_IDTS.
         apply ValueTPairSetFacts.filter_iff in MEM; [| solve_compat_bool ].
         des; des_bool; ss.
         unfold ValueTPair.get_idTs in *. ss.
-        apply list_inb_false_app in MEM0. des.
+        apply list_inb_false_app_inv in MEM0. des.
         erewrite <- clear_idt_spec_value in VAL1; ss.
         erewrite <- clear_idt_spec_value in VAL2; ss.
         eapply DIFFBLOCK; eauto.
@@ -297,7 +312,7 @@ Section CLEAR_IDTS.
         apply PtrPairSetFacts.filter_iff in MEM; [| solve_compat_bool ].
         des; des_bool; ss.
         unfold PtrPair.get_idTs in *. ss.
-        apply list_inb_false_app in MEM0. des.
+        apply list_inb_false_app_inv in MEM0. des.
         unfold Ptr.get_idTs in *. des_ifs. ss.
         erewrite <- clear_idt_spec_value in VAL1; ss.
         erewrite <- clear_idt_spec_value in VAL2; ss.
@@ -377,3 +392,461 @@ Section CLEAR_IDTS.
   Local Transparent InvState.Unary.clear_idt.
 
 End CLEAR_IDTS.
+
+
+
+
+Section CLEAR_IDTS_INV.
+
+  Lemma clear_idt_inv_spec_id
+        i0 idt0 st invst0
+        gv
+        (SOME: InvState.Unary.sem_idT st (InvState.Unary.clear_idt idt0 invst0) i0
+               = Some gv)
+        (NOTPHYSICAL: idt0.(fst) <> Tag.physical)
+    :
+      <<CLEAR: proj_sumbool (IdTSetFacts.eq_dec i0 idt0) = false>>
+  .
+  Proof.
+    red.
+    unfold InvState.Unary.clear_idt in *. des_ifs_safe. ss.
+    unfold proj_sumbool. des_ifs_safe.
+    destruct t; ss.
+    - unfold InvState.Unary.sem_idT, InvState.Unary.sem_tag in *. ss.
+      rewrite lookup_AL_filter_spec in SOME. unfold negb, proj_sumbool in *. des_ifs.
+    - unfold InvState.Unary.sem_idT, InvState.Unary.sem_tag in *. ss.
+      rewrite lookup_AL_filter_spec in SOME. unfold negb, proj_sumbool in *. des_ifs.
+  Qed.
+
+  Lemma clear_idt_inv_spec_value
+        v0 idt0 conf st invst0
+        gv
+        (SOME: InvState.Unary.sem_valueT conf st (InvState.Unary.clear_idt idt0 invst0) v0
+               = Some gv)
+        (NOTPHYSICAL: idt0.(fst) <> Tag.physical)
+    :
+      <<CLEAR: list_inb IdTSetFacts.eq_dec (ValueT.get_idTs v0) idt0 = false>>
+  .
+  Proof.
+    destruct v0; ss.
+    compute. des_ifs.
+    exploit clear_idt_inv_spec_id; try eassumption.
+    i; des. des_sumbool. ss.
+  Qed.
+
+  Lemma clear_idt_inv_spec_list_value
+        vs0 idt0 conf st invst0
+        gv
+        (SOME: InvState.Unary.sem_list_valueT conf st (InvState.Unary.clear_idt idt0 invst0) vs0
+               = Some gv)
+        (NOTPHYSICAL: idt0.(fst) <> Tag.physical)
+    :
+      <<CLEAR: list_inb IdTSetFacts.eq_dec (filter_map ValueT.get_idTs (List.map snd vs0))
+                        idt0 = false>>
+  .
+  Proof.
+    Local Opaque InvState.Unary.clear_idt.
+    destruct idt0; ss.
+    ginduction vs0; ii; ss.
+    des_ifs_safe. ss.
+    abstr (filter_map ValueT.get_idTs (List.map snd vs0)) tt.
+    exploit clear_idt_inv_spec_value; try eassumption. i.
+    destruct t0; ss; cycle 1.
+    { eapply IHvs0; eauto. }
+    replace (x :: tt) with ([x] ++ tt) by ss.
+    apply list_inb_false_app; cycle 1.
+    { eapply IHvs0; eauto. }
+    compute. des_ifs.
+  Qed.
+
+  Lemma clear_idt_inv_spec_expr
+        x idt0 conf st invst0
+        gv
+        (SOME: InvState.Unary.sem_expr conf st (InvState.Unary.clear_idt idt0 invst0) x
+               = Some gv)
+        (NOTPHYSICAL: idt0.(fst) <> Tag.physical)
+    :
+      <<CLEAR: list_inb IdTSetFacts.eq_dec (Expr.get_idTs x) idt0 = false>>
+  .
+  Proof.
+    Local Opaque filter_map.
+    red.
+    unfold Expr.get_idTs in *.
+    destruct x; ss.
+    - des_ifs_safe.
+      exploit clear_idt_inv_spec_value; try exact Heq; ss. intro IH0.
+      exploit clear_idt_inv_spec_value; try exact Heq0; ss. intro IH1.
+      eapply list_inb_filter_map_cons; eauto.
+    - des_ifs_safe.
+      exploit clear_idt_inv_spec_value; try exact Heq; ss. intro IH0.
+      exploit clear_idt_inv_spec_value; try exact Heq0; ss. intro IH1.
+      eapply list_inb_filter_map_cons; eauto.
+    - des_ifs_safe.
+      exploit clear_idt_inv_spec_value; try exact Heq; ss.
+    - des_ifs_safe.
+      exploit clear_idt_inv_spec_value; try exact Heq; ss. intro IH0.
+      exploit clear_idt_inv_spec_value; try exact Heq0; ss. intro IH1.
+      eapply list_inb_filter_map_cons; eauto.
+    - des_ifs_safe.
+      exploit clear_idt_inv_spec_value; try exact Heq; ss. intro IH0.
+      exploit clear_idt_inv_spec_list_value; try exact Heq0; ss. intro IH1.
+      eapply list_inb_filter_map_cons; eauto.
+    - des_ifs_safe.
+      exploit clear_idt_inv_spec_value; try exact Heq; ss.
+    - des_ifs_safe.
+      exploit clear_idt_inv_spec_value; try exact Heq; ss.
+    - des_ifs_safe.
+      exploit clear_idt_inv_spec_value; try exact Heq; ss.
+    - des_ifs_safe.
+      exploit clear_idt_inv_spec_value; try exact Heq; ss. intro IH0.
+      exploit clear_idt_inv_spec_value; try exact Heq0; ss. intro IH1.
+      eapply list_inb_filter_map_cons; eauto.
+    - des_ifs_safe.
+      exploit clear_idt_inv_spec_value; try exact Heq; ss. intro IH0.
+      exploit clear_idt_inv_spec_value; try exact Heq0; ss. intro IH1.
+      eapply list_inb_filter_map_cons; eauto.
+    - des_ifs_safe.
+      exploit clear_idt_inv_spec_value; try exact Heq; ss. intro IH0.
+      exploit clear_idt_inv_spec_value; try exact Heq0; ss. intro IH1.
+      exploit clear_idt_inv_spec_value; try exact Heq1; ss. intro IH2.
+      eapply list_inb_filter_map_cons; eauto.
+      eapply list_inb_filter_map_cons; eauto.
+    - des_ifs_safe.
+      exploit clear_idt_inv_spec_value; try exact SOME; ss.
+    - des_ifs_safe.
+      exploit clear_idt_inv_spec_value; try exact Heq; ss.
+  Qed.
+
+
+End CLEAR_IDTS_INV.
+  
+
+
+
+
+
+
+
+Section CONS_IDT.
+
+  Definition cons_idt_unary (idt0: IdT.t) (gv: GenericValue)
+             (inv0: InvState.Unary.t): InvState.Unary.t :=
+    match idt0.(fst) with
+    | Tag.physical => inv0
+    | Tag.previous => (InvState.Unary.update_previous
+                         (fun idgs => (idt0.(snd), gv) :: idgs) inv0)
+    | Tag.ghost => (InvState.Unary.update_ghost
+                      (fun idgs => (idt0.(snd), gv) :: idgs) inv0)
+    end
+  .
+
+  Definition cons_idt (idt0: IdT.t) (gv_src gv_tgt: GenericValue)
+             (inv0: InvState.Rel.t): InvState.Rel.t :=
+    InvState.Rel.mk (cons_idt_unary idt0 gv_src inv0.(InvState.Rel.src))
+                    (cons_idt_unary idt0 gv_tgt inv0.(InvState.Rel.tgt))
+  .
+
+  Lemma cons_idt_spec_id
+        i0 idt0
+        (CLEAR: proj_sumbool (IdTSetFacts.eq_dec i0 idt0) = false)
+        st invst0
+        gv0
+  :
+    <<EQ: InvState.Unary.sem_idT st invst0 i0 =
+          InvState.Unary.sem_idT st (cons_idt_unary idt0 gv0 invst0) i0>>
+  .
+  Proof.
+    red.
+    destruct idt0; ss.
+    unfold cons_idt_unary. ss.
+    unfold InvState.Unary.sem_idT.
+    unfold InvState.Unary.sem_tag.
+    destruct i0; ss.
+    des_sumbool.
+    destruct t, t0; ss; des_ifs.
+  Qed.
+
+  (* Lemma clear_idt_spec_inv_id *)
+  (*       i0 idt0 st_src invst0 *)
+  (*       gv *)
+  (*       (SOME: InvState.Unary.sem_idT st_src (InvState.Unary.clear_idt idt0 invst0) i0 *)
+  (*              = Some gv) *)
+  (*       (NOTPHYSICAL: idt0.(fst) <> Tag.physical) *)
+  (*   : *)
+  (*     (* <<NOTIN: idt0 <> i0>> *) *)
+  (*     <<CLEAR: proj_sumbool (IdTSetFacts.eq_dec i0 idt0) = false>> *)
+  (* . *)
+
+  Lemma cons_idt_spec_value
+        v0 idt0
+        (CLEAR: list_inb IdTSetFacts.eq_dec (ValueT.get_idTs v0) idt0 = false)
+        st conf invst0
+        gv0
+  :
+    <<EQ: InvState.Unary.sem_valueT conf st invst0 v0 =
+          InvState.Unary.sem_valueT conf st (cons_idt_unary idt0 gv0 invst0) v0>>
+  .
+  Proof.
+    red. unfold InvState.Unary.sem_valueT. des_ifs.
+    erewrite cons_idt_spec_id; eauto.
+    apply list_inb_single in CLEAR. des. des_sumbool.
+    unfold proj_sumbool. des_ifs.
+  Qed.
+
+  Lemma cons_idt_spec_list_value
+        vs0 idt0
+        (CLEAR: list_inb IdTSetFacts.eq_dec
+                         (filter_map ValueT.get_idTs (List.map snd vs0)) idt0 = false)
+        st conf invst0
+        gv0
+  :
+    <<EQ: InvState.Unary.sem_list_valueT conf st invst0 vs0 =
+          InvState.Unary.sem_list_valueT conf st (cons_idt_unary idt0 gv0 invst0) vs0>>
+  .
+  Proof.
+    red.
+    ginduction vs0; ii; ss; des_ifs_safe; clarify.
+    destruct t.
+    + erewrite <- cons_idt_spec_value; cycle 1.
+      { des_ifs. ss. clarify. eapply list_inb_false_sub; eauto. repeat econs; eauto. }
+      exploit IHvs0; try eassumption.
+      { instantiate (1:= idt0).
+        des_ifs. ss. clarify. eapply list_inb_false_sub; eauto. repeat econs; eauto.
+        eapply sublist_refl; eauto. }
+      intro IH. erewrite <- IH.
+      des_ifs.
+    + erewrite <- cons_idt_spec_value; cycle 1.
+      { des_ifs. }
+      exploit IHvs0; try eassumption.
+      intro IH. erewrite <- IH.
+      des_ifs.
+  Qed.
+
+  Lemma cons_idt_spec_expr
+        x idt0
+        (CLEAR: list_inb IdTSetFacts.eq_dec (Expr.get_idTs x) idt0 = false)
+        st conf invst0
+        gv0
+  :
+    <<EQ: InvState.Unary.sem_expr conf st invst0 x =
+          InvState.Unary.sem_expr conf st (cons_idt_unary idt0 gv0 invst0) x>>
+  .
+  Proof.
+    red.
+    unfold Expr.get_idTs in *.
+    destruct x; ss.
+    - repeat erewrite <- cons_idt_spec_value; ss.
+      { des_ifs. ss. eapply list_inb_false_sub; eauto. repeat econs; eauto. }
+      { des_ifs. ss. eapply list_inb_false_sub; eauto. repeat econs; eauto. }
+    - repeat erewrite <- cons_idt_spec_value; ss.
+      { des_ifs. ss. eapply list_inb_false_sub; eauto. repeat econs; eauto. }
+      { des_ifs. ss. eapply list_inb_false_sub; eauto. repeat econs; eauto. }
+    - repeat erewrite <- cons_idt_spec_value; ss.
+    - repeat erewrite <- cons_idt_spec_value; ss.
+      { des_ifs. ss. eapply list_inb_false_sub; eauto. repeat econs; eauto. }
+      { des_ifs. ss. eapply list_inb_false_sub; eauto. repeat econs; eauto. }
+    - repeat erewrite <- cons_idt_spec_value; ss.
+      repeat erewrite <- cons_idt_spec_list_value; ss.
+      { des_ifs. ss. eapply list_inb_false_sub; eauto. repeat econs; eauto.
+        eapply sublist_refl; eauto. }
+      { des_ifs. ss. eapply list_inb_false_sub; eauto. repeat econs; eauto. }
+    - repeat erewrite <- cons_idt_spec_value; ss.
+    - repeat erewrite <- cons_idt_spec_value; ss.
+    - repeat erewrite <- cons_idt_spec_value; ss.
+    - repeat erewrite <- cons_idt_spec_value; ss.
+      { des_ifs. ss. eapply list_inb_false_sub; eauto. repeat econs; eauto. }
+      { des_ifs. ss. eapply list_inb_false_sub; eauto. repeat econs; eauto. }
+    - repeat erewrite <- cons_idt_spec_value; ss.
+      { des_ifs. ss. eapply list_inb_false_sub; eauto. repeat econs; eauto. }
+      { des_ifs. ss. eapply list_inb_false_sub; eauto. repeat econs; eauto. }
+    - repeat erewrite <- cons_idt_spec_value; ss.
+      { des_ifs; ss; eapply list_inb_false_sub; eauto; repeat econs; eauto. }
+      { des_ifs; ss; eapply list_inb_false_sub; eauto; repeat econs; eauto. }
+      { des_ifs; ss; eapply list_inb_false_sub; eauto; repeat econs; eauto. }
+    - repeat erewrite <- cons_idt_spec_value; ss.
+    - repeat erewrite <- cons_idt_spec_value; ss.
+  Qed.
+
+  Local Opaque cons_idt_unary.
+  Local Opaque InvState.Unary.clear_idt.
+
+  Corollary cons_idt_expr_sim
+        x idt0 gv_res
+        conf st invst0
+        (SEM: InvState.Unary.sem_expr
+                conf st
+                (InvState.Unary.clear_idt idt0 invst0) x
+               = Some gv_res)
+        gv0
+    :
+      <<SEM: InvState.Unary.sem_expr
+               conf st
+               (cons_idt_unary idt0 gv0 (InvState.Unary.clear_idt idt0 invst0)) x
+               =
+               (* Some gv_res *)
+               (* This form is easier to use *)
+               InvState.Unary.sem_expr
+                 conf st
+                 (InvState.Unary.clear_idt idt0 invst0) x>>
+  .
+  Proof.
+    destruct idt0; ss.
+    destruct t; ss.
+    - erewrite <- cons_idt_spec_expr; try eassumption; ss.
+      eapply clear_idt_inv_spec_expr; ss; eauto.
+    - erewrite <- cons_idt_spec_expr; try eassumption; ss.
+      eapply clear_idt_inv_spec_expr; ss; eauto.
+  Qed.
+
+End CONS_IDT.
+
+
+Section SET_INV.
+
+  Lemma in_ExprPairSet_inv
+        e0 e1 idt0 eps
+        (IN: ExprPairSet.In (e0, e1)
+                            (ExprPairSet.clear_idt idt0 eps))
+        (NOTPHYS: idt0.(fst) <> Tag.physical)
+  :
+    <<CLEAR0: list_inb IdTSetFacts.eq_dec (Expr.get_idTs e0) idt0 = false>> /\
+    <<CLEAR1: list_inb IdTSetFacts.eq_dec (Expr.get_idTs e1) idt0 = false>>
+  .
+  Proof.
+    unfold ExprPairSet.clear_idt in IN.
+    eapply ExprPairSetFacts.filter_iff in IN; [ | solve_compat_bool ].
+    des; des_bool.
+    unfold ExprPair.get_idTs in *. ss.
+    apply list_inb_false_app_inv in IN0. des. ss.
+  Qed.
+
+  Lemma in_ValueTPairSet_inv
+        e0 e1 idt0 vps
+        (IN: ValueTPairSet.In (e0, e1)
+                            (ValueTPairSet.clear_idt idt0 vps))
+        (NOTPHYS: idt0.(fst) <> Tag.physical)
+  :
+    <<CLEAR0: list_inb IdTSetFacts.eq_dec (ValueT.get_idTs e0) idt0 = false>> /\
+    <<CLEAR1: list_inb IdTSetFacts.eq_dec (ValueT.get_idTs e1) idt0 = false>>
+  .
+  Proof.
+    unfold ValueTPairSet.clear_idt in IN.
+    eapply ValueTPairSetFacts.filter_iff in IN; [ | solve_compat_bool ].
+    des; des_bool.
+    unfold ValueTPair.get_idTs in *. ss.
+    apply list_inb_false_app_inv in IN0. des. ss.
+  Qed.
+
+  Lemma in_PtrPairSet_inv
+        e0 e1 idt0 vps
+        (IN: PtrPairSet.In (e0, e1)
+                            (PtrPairSet.clear_idt idt0 vps))
+        (NOTPHYS: idt0.(fst) <> Tag.physical)
+  :
+    <<CLEAR0: list_inb IdTSetFacts.eq_dec (Ptr.get_idTs e0) idt0 = false>> /\
+    <<CLEAR1: list_inb IdTSetFacts.eq_dec (Ptr.get_idTs e1) idt0 = false>>
+  .
+  Proof.
+    unfold PtrPairSet.clear_idt in IN.
+    eapply PtrPairSetFacts.filter_iff in IN; [ | solve_compat_bool ].
+    des; des_bool.
+    unfold PtrPair.get_idTs in *. ss.
+    apply list_inb_false_app_inv in IN0. des. ss.
+  Qed.
+
+  Lemma in_IdTSet_inv
+        e0 idt0 vps
+        (IN: IdTSet.In e0 (IdTSet.clear_idt idt0 vps))
+        (NOTPHYS: idt0.(fst) <> Tag.physical)
+    :
+      <<CLEAR: proj_sumbool (IdTSetFacts.eq_dec e0 idt0) = false>>
+  .
+  Proof.
+    unfold IdTSet.clear_idt in IN.
+    eapply IdTSetFacts.filter_iff in IN; [ | solve_compat_bool ].
+    des; des_bool.
+    des_sumbool. destruct idt0; ss. destruct e0; ss.
+    unfold proj_sumbool. des_ifs.
+  Qed.
+
+End SET_INV.
+
+Lemma cons_ghost_unary_spec
+      conf st x0 i0 gv
+      invst0 invmem0 gmax pubs inv0
+      (GV: InvState.Unary.sem_expr
+             conf st (InvState.Unary.clear_idt (Exprs.Tag.ghost, i0) invst0) x0 = Some gv)
+      (VALID: MemProps.valid_ptrs (Mem.nextblock (Mem st)) gv)
+      (SEM: InvState.Unary.sem conf st
+                               (InvState.Unary.clear_idt (Exprs.Tag.ghost, i0) invst0)
+                               invmem0 gmax pubs
+                               (Hints.Invariant.clear_idt_unary (Exprs.Tag.ghost, i0) inv0))
+  :
+    <<SEM: InvState.Unary.sem
+             conf st
+             (cons_idt_unary (Exprs.Tag.ghost, i0) gv
+                               (InvState.Unary.clear_idt (Exprs.Tag.ghost, i0) invst0))
+             invmem0 gmax
+             pubs
+             (Hints.Invariant.update_lessdef
+                ((Exprs.ExprPairSet.add
+                   (Exprs.Expr.value (Exprs.ValueT.id (Exprs.Tag.ghost, i0)), x0))
+                   <*>
+                   (Exprs.ExprPairSet.add
+                      (x0, Exprs.Expr.value (Exprs.ValueT.id (Exprs.Tag.ghost, i0)))))
+                (Hints.Invariant.clear_idt_unary (Exprs.Tag.ghost, i0) inv0))>>
+.
+Proof.
+  Local Opaque InvState.Unary.clear_idt.
+  econs; eauto; try apply SEM.
+  - inv SEM. clear - GV LESSDEF.
+    ii. ss.
+    apply ExprPairSetFacts.add_iff in H. des.
+    { clarify. ss.
+      compute in VAL1. des_ifs.
+      erewrite cons_idt_expr_sim; eauto.
+      esplits; eauto.
+      apply GVs.lessdef_refl.
+    }
+    apply ExprPairSetFacts.add_iff in H. des.
+    { clarify. ss.
+      erewrite cons_idt_expr_sim in VAL1; eauto. rewrite VAL1 in *. clarify.
+      exists gv; splits; ss.
+      - compute. des_ifs.
+      - apply GVs.lessdef_refl.
+    }
+    destruct x as [e0 e1]; ss.
+    exploit in_ExprPairSet_inv; try eassumption; ss. i; des.
+    erewrite <- cons_idt_spec_expr in VAL1; cycle 1; ss.
+    exploit LESSDEF; eauto. i; des.
+    esplits; eauto.
+    erewrite <- cons_idt_spec_expr; ss.
+  - inv SEM. clear - GV NOALIAS.
+    econs; eauto; ss.
+    + inv NOALIAS. clear - GV DIFFBLOCK.
+      i.
+      apply ValueTPairSetFacts.mem_iff in MEM.
+      exploit in_ValueTPairSet_inv; try eassumption; ss. i; des.
+      apply ValueTPairSetFacts.mem_iff in MEM.
+      erewrite <- cons_idt_spec_value in VAL1; cycle 1; ss.
+      erewrite <- cons_idt_spec_value in VAL2; cycle 1; ss.
+      eapply DIFFBLOCK; eauto.
+    + inv NOALIAS. clear - GV NOALIAS0.
+      i.
+      apply PtrPairSetFacts.mem_iff in MEM.
+      exploit in_PtrPairSet_inv; try eassumption; ss. i; des.
+      apply PtrPairSetFacts.mem_iff in MEM.
+      unfold Ptr.get_idTs in *. des_ifs_safe.
+      erewrite <- cons_idt_spec_value in VAL1; cycle 1; ss.
+      erewrite <- cons_idt_spec_value in VAL2; cycle 1; ss.
+      eapply NOALIAS0; eauto.
+  - inv SEM. clear - GV PRIVATE.
+    ss.
+    ii.
+    exploit in_IdTSet_inv; try eassumption; ss. i; des.
+    erewrite <- cons_idt_spec_id in VAL; cycle 1; ss.
+    eapply PRIVATE; eauto.
+  - inv SEM. clear - GV WF_GHOST VALID.
+    ii. ss. des_ifs.
+    + eapply WF_GHOST; eauto. 
+Qed.
